src/generated.c
@@ -290,127 +290,121 @@ _Bool is_well_chunk_bool(unsigned int chunk)
 
 unsigned char *check_mem_aux2(struct memory_region *mr$190, unsigned int perm, unsigned int addr, unsigned int chunk$196)
 {
-  _Bool well_chunk;
   unsigned int start;
   unsigned int size;
   unsigned int mr_perm;
   unsigned int lo_ofs;
   unsigned int hi_ofs;
-  well_chunk = is_well_chunk_bool(chunk$196);
-  if (well_chunk) {
-    start = get_start_addr(mr$190);
-    size = get_block_size(mr$190);
-    mr_perm = get_block_perm(mr$190);
-    lo_ofs = get_sub(addr, start);
-    hi_ofs = get_add(lo_ofs, chunk$196);
-    if (hi_ofs < size
-          && (lo_ofs <= 4294967295U - chunk$196 && 0U == lo_ofs % chunk$196)
-          && mr_perm >= perm) {
-      return (*mr$190).block_ptr + lo_ofs;
-    } else {
-      return 0;
-    }
+  start = get_start_addr(mr$190);
+  size = get_block_size(mr$190);
+  mr_perm = get_block_perm(mr$190);
+  lo_ofs = get_sub(addr, start);
+  hi_ofs = get_add(lo_ofs, chunk$196);
+  if (hi_ofs < size
+        && (lo_ofs <= 4294967295U - chunk$196 && 0U == lo_ofs % chunk$196)
+        && mr_perm >= perm) {
+    return (*mr$190).block_ptr + lo_ofs;
   } else {
     return 0;
   }
 }
 
-unsigned char *check_mem_aux(unsigned int num, unsigned int perm$212, unsigned int chunk$214, unsigned int addr$216, struct memory_region *mrs$218)
+unsigned char *check_mem_aux(unsigned int num, unsigned int perm$210, unsigned int chunk$212, unsigned int addr$214, struct memory_region *mrs$216)
 {
-  unsigned int n$220;
+  unsigned int n$218;
   struct memory_region *cur_mr;
-  unsigned char *check_mem$224;
+  unsigned char *check_mem$222;
   _Bool is_null;
   if (num == 0U) {
     return 0;
   } else {
-    n$220 = num - 1U;
-    cur_mr = get_mem_region(n$220, mrs$218);
-    check_mem$224 = check_mem_aux2(cur_mr, perm$212, addr$216, chunk$214);
-    is_null = cmp_ptr32_nullM(check_mem$224);
+    n$218 = num - 1U;
+    cur_mr = get_mem_region(n$218, mrs$216);
+    check_mem$222 = check_mem_aux2(cur_mr, perm$210, addr$214, chunk$212);
+    is_null = cmp_ptr32_nullM(check_mem$222);
     if (is_null) {
-      return check_mem_aux(n$220, perm$212, chunk$214, addr$216, mrs$218);
+      return check_mem_aux(n$218, perm$210, chunk$212, addr$214, mrs$216);
     } else {
-      return check_mem$224;
+      return check_mem$222;
     }
   }
 }
 
-unsigned char *check_mem(unsigned int perm$228, unsigned int chunk$230, unsigned int addr$232)
+unsigned char *check_mem(unsigned int perm$226, unsigned int chunk$228, unsigned int addr$230)
 {
-  _Bool well_chunk$234;
+  _Bool well_chunk;
   unsigned int mem_reg_num;
-  struct memory_region *mrs$238;
-  unsigned char *check_mem$240;
-  _Bool is_null$242;
-  well_chunk$234 = is_well_chunk_bool(chunk$230);
-  if (well_chunk$234) {
+  struct memory_region *mrs$236;
+  unsigned char *check_mem$238;
+  _Bool is_null$240;
+  well_chunk = is_well_chunk_bool(chunk$228);
+  if (well_chunk) {
     mem_reg_num = eval_mrs_num();
-    mrs$238 = eval_mrs_regions();
-    check_mem$240 =
-      check_mem_aux(mem_reg_num, perm$228, chunk$230, addr$232, mrs$238);
-    is_null$242 = cmp_ptr32_nullM(check_mem$240);
-    if (is_null$242) {
+    mrs$236 = eval_mrs_regions();
+    check_mem$238 =
+      check_mem_aux(mem_reg_num, perm$226, chunk$228, addr$230, mrs$236);
+    is_null$240 = cmp_ptr32_nullM(check_mem$238);
+    if (is_null$240) {
       return 0;
     } else {
-      return check_mem$240;
+      return check_mem$238;
     }
   } else {
     return 0;
   }
 }
 
-void step_opcode_alu64(unsigned long long dst64, unsigned long long src64$246, unsigned int dst, unsigned char op$250)
+void step_opcode_alu64(unsigned long long dst64, unsigned long long src64$244, unsigned int dst, unsigned char op$248)
 {
   unsigned char opcode_alu64;
+  unsigned int src32$252;
   unsigned int src32$254;
   unsigned int src32$256;
-  unsigned int src32$258;
-  opcode_alu64 = get_opcode_alu64(op$250);
+  opcode_alu64 = get_opcode_alu64(op$248);
   switch (opcode_alu64) {
     case 0:
-      upd_reg(dst, dst64 + src64$246);
+      upd_reg(dst, dst64 + src64$244);
       return;
     case 16:
-      upd_reg(dst, dst64 - src64$246);
+      upd_reg(dst, dst64 - src64$244);
       return;
     case 32:
-      upd_reg(dst, dst64 * src64$246);
+      upd_reg(dst, dst64 * src64$244);
       return;
     case 48:
-      if (src64$246 != 0LLU) {
-        upd_reg(dst, dst64 / src64$246);
+      if (src64$244 != 0LLU) {
+        upd_reg(dst, dst64 / src64$244);
         return;
       } else {
         upd_flag(-9);
         return;
       }
     case 64:
-      upd_reg(dst, dst64 | src64$246);
+      upd_reg(dst, dst64 | src64$244);
       return;
     case 80:
-      upd_reg(dst, dst64 & src64$246);
+      upd_reg(dst, dst64 & src64$244);
       return;
     case 96:
-      src32$254 = reg64_to_reg32(src64$246);
-      if (src32$254 < 64U) {
-        upd_reg(dst, dst64 << src32$254);
+      src32$252 = reg64_to_reg32(src64$244);
+      if (src32$252 < 64U) {
+        upd_reg(dst, dst64 << src32$252);
         return;
       } else {
         upd_flag(-10);
         return;
       }
     case 112:
-      src32$256 = reg64_to_reg32(src64$246);
-      if (src32$256 < 64U) {
-        upd_reg(dst, dst64 >> src32$256);
+      src32$254 = reg64_to_reg32(src64$244);
+      if (src32$254 < 64U) {
+        upd_reg(dst, dst64 >> src32$254);
         return;
       } else {
         upd_flag(-10);
         return;
       }
     case 128:
-      if (op$250 == 135) {
+      if (op$248 == 135) {
         upd_reg(dst, -dst64);
         return;
       } else {
@@ -418,23 +412,23 @@ void step_opcode_alu64(unsigned long long dst64, unsigned long long src64$246, u
         return;
       }
     case 144:
-      if (src64$246 != 0LLU) {
-        upd_reg(dst, dst64 % src64$246);
+      if (src64$244 != 0LLU) {
+        upd_reg(dst, dst64 % src64$244);
         return;
       } else {
         upd_flag(-9);
         return;
       }
     case 160:
-      upd_reg(dst, dst64 ^ src64$246);
+      upd_reg(dst, dst64 ^ src64$244);
       return;
     case 176:
-      upd_reg(dst, src64$246);
+      upd_reg(dst, src64$244);
       return;
     case 192:
-      src32$258 = reg64_to_reg32(src64$246);
-      if (src32$258 < 64U) {
-        upd_reg(dst, (unsigned long long) ((long long) dst64 >> src32$258));
+      src32$256 = reg64_to_reg32(src64$244);
+      if (src32$256 < 64U) {
+        upd_reg(dst, (unsigned long long) ((long long) dst64 >> src32$256));
         return;
       } else {
         upd_flag(-10);
@@ -447,75 +441,75 @@ void step_opcode_alu64(unsigned long long dst64, unsigned long long src64$246, u
   }
 }
 
-void step_opcode_alu32(unsigned int dst32, unsigned int src32$262, unsigned int dst$264, unsigned char op$266)
+void step_opcode_alu32(unsigned int dst32, unsigned int src32$260, unsigned int dst$262, unsigned char op$264)
 {
   unsigned char opcode_alu32;
-  opcode_alu32 = get_opcode_alu32(op$266);
+  opcode_alu32 = get_opcode_alu32(op$264);
   switch (opcode_alu32) {
     case 0:
-      upd_reg(dst$264, (unsigned long long) (dst32 + src32$262));
+      upd_reg(dst$262, (unsigned long long) (dst32 + src32$260));
       return;
     case 16:
-      upd_reg(dst$264, (unsigned long long) (dst32 - src32$262));
+      upd_reg(dst$262, (unsigned long long) (dst32 - src32$260));
       return;
     case 32:
-      upd_reg(dst$264, (unsigned long long) (dst32 * src32$262));
+      upd_reg(dst$262, (unsigned long long) (dst32 * src32$260));
       return;
     case 48:
-      if (src32$262 != 0U) {
-        upd_reg(dst$264, (unsigned long long) (dst32 / src32$262));
+      if (src32$260 != 0U) {
+        upd_reg(dst$262, (unsigned long long) (dst32 / src32$260));
         return;
       } else {
         upd_flag(-9);
         return;
       }
     case 64:
-      upd_reg(dst$264, (unsigned long long) (dst32 | src32$262));
+      upd_reg(dst$262, (unsigned long long) (dst32 | src32$260));
       return;
     case 80:
-      upd_reg(dst$264, (unsigned long long) (dst32 & src32$262));
+      upd_reg(dst$262, (unsigned long long) (dst32 & src32$260));
       return;
     case 96:
-      if (src32$262 < 32U) {
-        upd_reg(dst$264, (unsigned long long) (dst32 << src32$262));
+      if (src32$260 < 32U) {
+        upd_reg(dst$262, (unsigned long long) (dst32 << src32$260));
         return;
       } else {
         upd_flag(-10);
         return;
       }
     case 112:
-      if (src32$262 < 32U) {
-        upd_reg(dst$264, (unsigned long long) (dst32 >> src32$262));
+      if (src32$260 < 32U) {
+        upd_reg(dst$262, (unsigned long long) (dst32 >> src32$260));
         return;
       } else {
         upd_flag(-10);
         return;
       }
     case 128:
-      if (op$266 == 132) {
-        upd_reg(dst$264, (unsigned long long) -dst32);
+      if (op$264 == 132) {
+        upd_reg(dst$262, (unsigned long long) -dst32);
         return;
       } else {
         upd_flag(-1);
         return;
       }
     case 144:
-      if (src32$262 != 0U) {
-        upd_reg(dst$264, (unsigned long long) (dst32 % src32$262));
+      if (src32$260 != 0U) {
+        upd_reg(dst$262, (unsigned long long) (dst32 % src32$260));
         return;
       } else {
         upd_flag(-9);
         return;
       }
     case 160:
-      upd_reg(dst$264, (unsigned long long) (dst32 ^ src32$262));
+      upd_reg(dst$262, (unsigned long long) (dst32 ^ src32$260));
       return;
     case 176:
-      upd_reg(dst$264, (unsigned long long) src32$262);
+      upd_reg(dst$262, (unsigned long long) src32$260);
       return;
     case 192:
-      if (src32$262 < 32U) {
-        upd_reg(dst$264, (unsigned long long) ((int) dst32 >> src32$262));
+      if (src32$260 < 32U) {
+        upd_reg(dst$262, (unsigned long long) ((int) dst32 >> src32$260));
         return;
       } else {
         upd_flag(-10);
@@ -528,104 +522,104 @@ void step_opcode_alu32(unsigned int dst32, unsigned int src32$262, unsigned int 
   }
 }
 
-void step_opcode_branch(unsigned long long dst64$270, unsigned long long src64$272, int pc, int ofs$276, unsigned char op$278)
+void step_opcode_branch(unsigned long long dst64$268, unsigned long long src64$270, int pc, int ofs$274, unsigned char op$276)
 {
   unsigned char opcode_jmp;
   unsigned char *f_ptr;
-  _Bool is_null$284;
+  _Bool is_null$282;
   unsigned int res;
-  opcode_jmp = get_opcode_branch(op$278);
+  opcode_jmp = get_opcode_branch(op$276);
   switch (opcode_jmp) {
     case 0:
-      if (op$278 == 5) {
-        upd_pc(pc + ofs$276);
+      if (op$276 == 5) {
+        upd_pc(pc + ofs$274);
         return;
       } else {
         upd_flag(-1);
         return;
       }
     case 16:
-      if (dst64$270 == src64$272) {
-        upd_pc(pc + ofs$276);
+      if (dst64$268 == src64$270) {
+        upd_pc(pc + ofs$274);
         return;
       } else {
         return;
       }
     case 32:
-      if (dst64$270 > src64$272) {
-        upd_pc(pc + ofs$276);
+      if (dst64$268 > src64$270) {
+        upd_pc(pc + ofs$274);
         return;
       } else {
         return;
       }
     case 48:
-      if (dst64$270 >= src64$272) {
-        upd_pc(pc + ofs$276);
+      if (dst64$268 >= src64$270) {
+        upd_pc(pc + ofs$274);
         return;
       } else {
         return;
       }
     case 160:
-      if (dst64$270 < src64$272) {
-        upd_pc(pc + ofs$276);
+      if (dst64$268 < src64$270) {
+        upd_pc(pc + ofs$274);
         return;
       } else {
         return;
       }
     case 176:
-      if (dst64$270 <= src64$272) {
-        upd_pc(pc + ofs$276);
+      if (dst64$268 <= src64$270) {
+        upd_pc(pc + ofs$274);
         return;
       } else {
         return;
       }
     case 64:
-      if ((dst64$270 & src64$272) != 0LLU) {
-        upd_pc(pc + ofs$276);
+      if ((dst64$268 & src64$270) != 0LLU) {
+        upd_pc(pc + ofs$274);
         return;
       } else {
         return;
       }
     case 80:
-      if (dst64$270 != src64$272) {
-        upd_pc(pc + ofs$276);
+      if (dst64$268 != src64$270) {
+        upd_pc(pc + ofs$274);
         return;
       } else {
         return;
       }
     case 96:
-      if ((long long) dst64$270 > (long long) src64$272) {
-        upd_pc(pc + ofs$276);
+      if ((long long) dst64$268 > (long long) src64$270) {
+        upd_pc(pc + ofs$274);
         return;
       } else {
         return;
       }
     case 112:
-      if ((long long) dst64$270 >= (long long) src64$272) {
-        upd_pc(pc + ofs$276);
+      if ((long long) dst64$268 >= (long long) src64$270) {
+        upd_pc(pc + ofs$274);
         return;
       } else {
         return;
       }
     case 192:
-      if ((long long) dst64$270 < (long long) src64$272) {
-        upd_pc(pc + ofs$276);
+      if ((long long) dst64$268 < (long long) src64$270) {
+        upd_pc(pc + ofs$274);
         return;
       } else {
         return;
       }
     case 208:
-      if ((long long) dst64$270 <= (long long) src64$272) {
-        upd_pc(pc + ofs$276);
+      if ((long long) dst64$268 <= (long long) src64$270) {
+        upd_pc(pc + ofs$274);
         return;
       } else {
         return;
       }
     case 128:
-      if (op$278 == 133) {
-        f_ptr = _bpf_get_call((int) src64$272);
-        is_null$284 = cmp_ptr32_nullM(f_ptr);
-        if (is_null$284) {
+      if (op$276 == 133) {
+        f_ptr = _bpf_get_call((int) src64$270);
+        is_null$282 = cmp_ptr32_nullM(f_ptr);
+        if (is_null$282) {
           upd_flag(-4);
           return;
         } else {
@@ -638,7 +632,7 @@ void step_opcode_branch(unsigned long long dst64$270, unsigned long long src64$2
         return;
       }
     case 144:
-      if (op$278 == 149) {
+      if (op$276 == 149) {
         upd_flag(1);
         return;
       } else {
@@ -652,21 +646,21 @@ void step_opcode_branch(unsigned long long dst64$270, unsigned long long src64$2
   }
 }
 
-void step_opcode_mem_ld_imm(int imm$288, int pc$290, unsigned int dst$292, unsigned char op$294)
+void step_opcode_mem_ld_imm(int imm$286, int pc$288, unsigned int dst$290, unsigned char op$292)
 {
   int len;
   unsigned char opcode_ld;
   unsigned long long next_ins;
   int next_imm;
   len = eval_ins_len();
-  opcode_ld = get_opcode_mem_ld_imm(op$294);
+  opcode_ld = get_opcode_mem_ld_imm(op$292);
   switch (opcode_ld) {
     case 24:
-      if (pc$290 + 1 < len) {
-        next_ins = eval_ins(pc$290 + 1);
+      if (pc$288 + 1 < len) {
+        next_ins = eval_ins(pc$288 + 1);
         next_imm = get_immediate(next_ins);
-        upd_reg(dst$292,
-                (unsigned long long) imm$288
+        upd_reg(dst$290,
+                (unsigned long long) imm$286
                   | (unsigned long long) next_imm << 32U);
         upd_pc_incr();
         return;
@@ -681,65 +675,65 @@ void step_opcode_mem_ld_imm(int imm$288, int pc$290, unsigned int dst$292, unsig
   }
 }
 
-void step_opcode_mem_ld_reg(unsigned int addr$304, int pc$306, unsigned int dst$308, unsigned char op$310)
+void step_opcode_mem_ld_reg(unsigned int addr$302, int pc$304, unsigned int dst$306, unsigned char op$308)
 {
-  unsigned char opcode_ld$312;
+  unsigned char opcode_ld$310;
   unsigned char *addr_ptr;
-  _Bool is_null$316;
+  _Bool is_null$314;
   unsigned long long v;
-  unsigned char *addr_ptr$320;
-  _Bool is_null$322;
-  unsigned long long v$324;
-  unsigned char *addr_ptr$326;
-  _Bool is_null$328;
-  unsigned long long v$330;
-  unsigned char *addr_ptr$332;
-  _Bool is_null$334;
-  unsigned long long v$336;
-  opcode_ld$312 = get_opcode_mem_ld_reg(op$310);
-  switch (opcode_ld$312) {
+  unsigned char *addr_ptr$318;
+  _Bool is_null$320;
+  unsigned long long v$322;
+  unsigned char *addr_ptr$324;
+  _Bool is_null$326;
+  unsigned long long v$328;
+  unsigned char *addr_ptr$330;
+  _Bool is_null$332;
+  unsigned long long v$334;
+  opcode_ld$310 = get_opcode_mem_ld_reg(op$308);
+  switch (opcode_ld$310) {
     case 97:
-      addr_ptr = check_mem(1U, 4U, addr$304);
-      is_null$316 = cmp_ptr32_nullM(addr_ptr);
-      if (is_null$316) {
+      addr_ptr = check_mem(1U, 4U, addr$302);
+      is_null$314 = cmp_ptr32_nullM(addr_ptr);
+      if (is_null$314) {
         upd_flag(-2);
         return;
       } else {
         v = load_mem(4U, addr_ptr);
-        upd_reg(dst$308, v);
+        upd_reg(dst$306, v);
         return;
       }
     case 105:
-      addr_ptr$320 = check_mem(1U, 2U, addr$304);
-      is_null$322 = cmp_ptr32_nullM(addr_ptr$320);
-      if (is_null$322) {
+      addr_ptr$318 = check_mem(1U, 2U, addr$302);
+      is_null$320 = cmp_ptr32_nullM(addr_ptr$318);
+      if (is_null$320) {
         upd_flag(-2);
         return;
       } else {
-        v$324 = load_mem(2U, addr_ptr$320);
-        upd_reg(dst$308, v$324);
+        v$322 = load_mem(2U, addr_ptr$318);
+        upd_reg(dst$306, v$322);
         return;
       }
     case 113:
-      addr_ptr$326 = check_mem(1U, 1U, addr$304);
-      is_null$328 = cmp_ptr32_nullM(addr_ptr$326);
-      if (is_null$328) {
+      addr_ptr$324 = check_mem(1U, 1U, addr$302);
+      is_null$326 = cmp_ptr32_nullM(addr_ptr$324);
+      if (is_null$326) {
         upd_flag(-2);
         return;
       } else {
-        v$330 = load_mem(1U, addr_ptr$326);
-        upd_reg(dst$308, v$330);
+        v$328 = load_mem(1U, addr_ptr$324);
+        upd_reg(dst$306, v$328);
         return;
       }
     case 121:
-      addr_ptr$332 = check_mem(1U, 8U, addr$304);
-      is_null$334 = cmp_ptr32_nullM(addr_ptr$332);
-      if (is_null$334) {
+      addr_ptr$330 = check_mem(1U, 8U, addr$302);
+      is_null$332 = cmp_ptr32_nullM(addr_ptr$330);
+      if (is_null$332) {
         upd_flag(-2);
         return;
       } else {
-        v$336 = load_mem(8U, addr_ptr$332);
-        upd_reg(dst$308, v$336);
+        v$334 = load_mem(8U, addr_ptr$330);
+        upd_reg(dst$306, v$334);
         return;
       }
     default:
@@ -749,57 +743,57 @@ void step_opcode_mem_ld_reg(unsigned int addr$304, int pc$306, unsigned int dst$
   }
 }
 
-void step_opcode_mem_st_imm(int imm$338, unsigned int addr$340, int pc$342, unsigned int dst$344, unsigned char op$346)
+void step_opcode_mem_st_imm(int imm$336, unsigned int addr$338, int pc$340, unsigned int dst$342, unsigned char op$344)
 {
   unsigned char opcode_st;
-  unsigned char *addr_ptr$350;
-  _Bool is_null$352;
-  unsigned char *addr_ptr$354;
-  _Bool is_null$356;
-  unsigned char *addr_ptr$358;
-  _Bool is_null$360;
-  unsigned char *addr_ptr$362;
-  _Bool is_null$364;
-  opcode_st = get_opcode_mem_st_imm(op$346);
+  unsigned char *addr_ptr$348;
+  _Bool is_null$350;
+  unsigned char *addr_ptr$352;
+  _Bool is_null$354;
+  unsigned char *addr_ptr$356;
+  _Bool is_null$358;
+  unsigned char *addr_ptr$360;
+  _Bool is_null$362;
+  opcode_st = get_opcode_mem_st_imm(op$344);
   switch (opcode_st) {
     case 98:
-      addr_ptr$350 = check_mem(2U, 4U, addr$340);
-      is_null$352 = cmp_ptr32_nullM(addr_ptr$350);
-      if (is_null$352) {
+      addr_ptr$348 = check_mem(2U, 4U, addr$338);
+      is_null$350 = cmp_ptr32_nullM(addr_ptr$348);
+      if (is_null$350) {
         upd_flag(-2);
         return;
       } else {
-        store_mem_imm(4U, addr_ptr$350, imm$338);
+        store_mem_imm(4U, addr_ptr$348, imm$336);
         return;
       }
     case 106:
-      addr_ptr$354 = check_mem(2U, 2U, addr$340);
-      is_null$356 = cmp_ptr32_nullM(addr_ptr$354);
-      if (is_null$356) {
+      addr_ptr$352 = check_mem(2U, 2U, addr$338);
+      is_null$354 = cmp_ptr32_nullM(addr_ptr$352);
+      if (is_null$354) {
         upd_flag(-2);
         return;
       } else {
-        store_mem_imm(2U, addr_ptr$354, imm$338);
+        store_mem_imm(2U, addr_ptr$352, imm$336);
         return;
       }
     case 114:
-      addr_ptr$358 = check_mem(2U, 1U, addr$340);
-      is_null$360 = cmp_ptr32_nullM(addr_ptr$358);
-      if (is_null$360) {
+      addr_ptr$356 = check_mem(2U, 1U, addr$338);
+      is_null$358 = cmp_ptr32_nullM(addr_ptr$356);
+      if (is_null$358) {
         upd_flag(-2);
         return;
       } else {
-        store_mem_imm(1U, addr_ptr$358, imm$338);
+        store_mem_imm(1U, addr_ptr$356, imm$336);
         return;
       }
     case 122:
-      addr_ptr$362 = check_mem(2U, 8U, addr$340);
-      is_null$364 = cmp_ptr32_nullM(addr_ptr$362);
-      if (is_null$364) {
+      addr_ptr$360 = check_mem(2U, 8U, addr$338);
+      is_null$362 = cmp_ptr32_nullM(addr_ptr$360);
+      if (is_null$362) {
         upd_flag(-2);
         return;
       } else {
-        store_mem_imm(8U, addr_ptr$362, imm$338);
+        store_mem_imm(8U, addr_ptr$360, imm$336);
         return;
       }
     default:
@@ -809,57 +803,57 @@ void step_opcode_mem_st_imm(int imm$338, unsigned int addr$340, int pc$342, unsi
   }
 }
 
-void step_opcode_mem_st_reg(unsigned long long src64$366, unsigned int addr$368, int pc$370, unsigned int dst$372, unsigned char op$374)
+void step_opcode_mem_st_reg(unsigned long long src64$364, unsigned int addr$366, int pc$368, unsigned int dst$370, unsigned char op$372)
 {
-  unsigned char opcode_st$376;
-  unsigned char *addr_ptr$378;
-  _Bool is_null$380;
-  unsigned char *addr_ptr$382;
-  _Bool is_null$384;
-  unsigned char *addr_ptr$386;
-  _Bool is_null$388;
-  unsigned char *addr_ptr$390;
-  _Bool is_null$392;
-  opcode_st$376 = get_opcode_mem_st_reg(op$374);
-  switch (opcode_st$376) {
+  unsigned char opcode_st$374;
+  unsigned char *addr_ptr$376;
+  _Bool is_null$378;
+  unsigned char *addr_ptr$380;
+  _Bool is_null$382;
+  unsigned char *addr_ptr$384;
+  _Bool is_null$386;
+  unsigned char *addr_ptr$388;
+  _Bool is_null$390;
+  opcode_st$374 = get_opcode_mem_st_reg(op$372);
+  switch (opcode_st$374) {
     case 99:
-      addr_ptr$378 = check_mem(2U, 4U, addr$368);
-      is_null$380 = cmp_ptr32_nullM(addr_ptr$378);
-      if (is_null$380) {
+      addr_ptr$376 = check_mem(2U, 4U, addr$366);
+      is_null$378 = cmp_ptr32_nullM(addr_ptr$376);
+      if (is_null$378) {
         upd_flag(-2);
         return;
       } else {
-        store_mem_reg(4U, addr_ptr$378, src64$366);
+        store_mem_reg(4U, addr_ptr$376, src64$364);
         return;
       }
     case 107:
-      addr_ptr$382 = check_mem(2U, 2U, addr$368);
-      is_null$384 = cmp_ptr32_nullM(addr_ptr$382);
-      if (is_null$384) {
+      addr_ptr$380 = check_mem(2U, 2U, addr$366);
+      is_null$382 = cmp_ptr32_nullM(addr_ptr$380);
+      if (is_null$382) {
         upd_flag(-2);
         return;
       } else {
-        store_mem_reg(2U, addr_ptr$382, src64$366);
+        store_mem_reg(2U, addr_ptr$380, src64$364);
         return;
       }
     case 115:
-      addr_ptr$386 = check_mem(2U, 1U, addr$368);
-      is_null$388 = cmp_ptr32_nullM(addr_ptr$386);
-      if (is_null$388) {
+      addr_ptr$384 = check_mem(2U, 1U, addr$366);
+      is_null$386 = cmp_ptr32_nullM(addr_ptr$384);
+      if (is_null$386) {
         upd_flag(-2);
         return;
       } else {
-        store_mem_reg(1U, addr_ptr$386, src64$366);
+        store_mem_reg(1U, addr_ptr$384, src64$364);
         return;
       }
     case 123:
-      addr_ptr$390 = check_mem(2U, 8U, addr$368);
-      is_null$392 = cmp_ptr32_nullM(addr_ptr$390);
-      if (is_null$392) {
+      addr_ptr$388 = check_mem(2U, 8U, addr$366);
+      is_null$390 = cmp_ptr32_nullM(addr_ptr$388);
+      if (is_null$390) {
         upd_flag(-2);
         return;
       } else {
-        store_mem_reg(8U, addr_ptr$390, src64$366);
+        store_mem_reg(8U, addr_ptr$388, src64$364);
         return;
       }
     default:
@@ -871,81 +865,81 @@ void step_opcode_mem_st_reg(unsigned long long src64$366, unsigned int addr$368,
 
 void step(void)
 {
-  int pc$394;
-  unsigned long long ins$396;
-  unsigned char op$398;
+  int pc$392;
+  unsigned long long ins$394;
+  unsigned char op$396;
   unsigned char opc;
-  unsigned int dst$402;
-  unsigned long long dst64$404;
-  unsigned long long src64$406;
-  unsigned long long dst64$408;
-  unsigned int dst32$410;
-  unsigned int src32$412;
-  unsigned long long dst64$414;
-  int ofs$416;
-  unsigned long long src64$418;
-  int imm$420;
-  unsigned int src$422;
-  unsigned long long src64$424;
-  int ofs$426;
-  unsigned int addr$428;
-  unsigned long long dst64$430;
-  int ofs$432;
-  int imm$434;
-  unsigned int addr$436;
-  unsigned long long dst64$438;
-  unsigned int src$440;
-  unsigned long long src64$442;
-  int ofs$444;
-  unsigned int addr$446;
-  pc$394 = eval_pc();
-  ins$396 = eval_ins(pc$394);
-  op$398 = get_opcode_ins(ins$396);
-  opc = get_opcode(op$398);
-  dst$402 = get_dst(ins$396);
+  unsigned int dst$400;
+  unsigned long long dst64$402;
+  unsigned long long src64$404;
+  unsigned long long dst64$406;
+  unsigned int dst32$408;
+  unsigned int src32$410;
+  unsigned long long dst64$412;
+  int ofs$414;
+  unsigned long long src64$416;
+  int imm$418;
+  unsigned int src$420;
+  unsigned long long src64$422;
+  int ofs$424;
+  unsigned int addr$426;
+  unsigned long long dst64$428;
+  int ofs$430;
+  int imm$432;
+  unsigned int addr$434;
+  unsigned long long dst64$436;
+  unsigned int src$438;
+  unsigned long long src64$440;
+  int ofs$442;
+  unsigned int addr$444;
+  pc$392 = eval_pc();
+  ins$394 = eval_ins(pc$392);
+  op$396 = get_opcode_ins(ins$394);
+  opc = get_opcode(op$396);
+  dst$400 = get_dst(ins$394);
   switch (opc) {
     case 7:
-      dst64$404 = eval_reg(dst$402);
-      src64$406 = get_src64(op$398, ins$396);
-      step_opcode_alu64(dst64$404, src64$406, dst$402, op$398);
+      dst64$402 = eval_reg(dst$400);
+      src64$404 = get_src64(op$396, ins$394);
+      step_opcode_alu64(dst64$402, src64$404, dst$400, op$396);
       return;
     case 4:
-      dst64$408 = eval_reg(dst$402);
-      dst32$410 = reg64_to_reg32(dst64$408);
-      src32$412 = get_src32(op$398, ins$396);
-      step_opcode_alu32(dst32$410, src32$412, dst$402, op$398);
+      dst64$406 = eval_reg(dst$400);
+      dst32$408 = reg64_to_reg32(dst64$406);
+      src32$410 = get_src32(op$396, ins$394);
+      step_opcode_alu32(dst32$408, src32$410, dst$400, op$396);
       return;
     case 5:
-      dst64$414 = eval_reg(dst$402);
-      ofs$416 = get_offset(ins$396);
-      src64$418 = get_src64(op$398, ins$396);
-      step_opcode_branch(dst64$414, src64$418, pc$394, ofs$416, op$398);
+      dst64$412 = eval_reg(dst$400);
+      ofs$414 = get_offset(ins$394);
+      src64$416 = get_src64(op$396, ins$394);
+      step_opcode_branch(dst64$412, src64$416, pc$392, ofs$414, op$396);
       return;
     case 0:
-      imm$420 = get_immediate(ins$396);
-      step_opcode_mem_ld_imm(imm$420, pc$394, dst$402, op$398);
+      imm$418 = get_immediate(ins$394);
+      step_opcode_mem_ld_imm(imm$418, pc$392, dst$400, op$396);
       return;
     case 1:
-      src$422 = get_src(ins$396);
-      src64$424 = eval_reg(src$422);
-      ofs$426 = get_offset(ins$396);
-      addr$428 = get_addr_ofs(src64$424, ofs$426);
-      step_opcode_mem_ld_reg(addr$428, pc$394, dst$402, op$398);
+      src$420 = get_src(ins$394);
+      src64$422 = eval_reg(src$420);
+      ofs$424 = get_offset(ins$394);
+      addr$426 = get_addr_ofs(src64$422, ofs$424);
+      step_opcode_mem_ld_reg(addr$426, pc$392, dst$400, op$396);
       return;
     case 2:
-      dst64$430 = eval_reg(dst$402);
-      ofs$432 = get_offset(ins$396);
-      imm$434 = get_immediate(ins$396);
-      addr$436 = get_addr_ofs(dst64$430, ofs$432);
-      step_opcode_mem_st_imm(imm$434, addr$436, pc$394, dst$402, op$398);
+      dst64$428 = eval_reg(dst$400);
+      ofs$430 = get_offset(ins$394);
+      imm$432 = get_immediate(ins$394);
+      addr$434 = get_addr_ofs(dst64$428, ofs$430);
+      step_opcode_mem_st_imm(imm$432, addr$434, pc$392, dst$400, op$396);
       return;
     case 3:
-      dst64$438 = eval_reg(dst$402);
-      src$440 = get_src(ins$396);
-      src64$442 = eval_reg(src$440);
-      ofs$444 = get_offset(ins$396);
-      addr$446 = get_addr_ofs(dst64$438, ofs$444);
-      step_opcode_mem_st_reg(src64$442, addr$446, pc$394, dst$402, op$398);
+      dst64$436 = eval_reg(dst$400);
+      src$438 = get_src(ins$394);
+      src64$440 = eval_reg(src$438);
+      ofs$442 = get_offset(ins$394);
+      addr$444 = get_addr_ofs(dst64$436, ofs$442);
+      step_opcode_mem_st_reg(src64$440, addr$444, pc$392, dst$400, op$396);
       return;
     default:
       upd_flag(-1);
@@ -957,17 +951,17 @@ void step(void)
 void bpf_interpreter_aux(unsigned int fuel)
 {
   unsigned int fuel0;
-  int len$452;
-  int pc$454;
+  int len$450;
+  int pc$452;
   int f;
   if (fuel == 0U) {
     upd_flag(-5);
     return;
   } else {
     fuel0 = fuel - 1U;
-    len$452 = eval_ins_len();
-    pc$454 = eval_pc();
-    if (0U <= pc$454 && pc$454 < len$452) {
+    len$450 = eval_ins_len();
+    pc$452 = eval_pc();
+    if (0U <= pc$452 && pc$452 < len$450) {
       step();
       f = eval_flag();
       if (f == 0) {
@@ -984,17 +978,17 @@ void bpf_interpreter_aux(unsigned int fuel)
   }
 }
 
-unsigned long long bpf_interpreter(unsigned int fuel$458)
+unsigned long long bpf_interpreter(unsigned int fuel$456)
 {
-  struct memory_region *mrs$460;
+  struct memory_region *mrs$458;
   struct memory_region *bpf_ctx;
-  int f$464;
-  mrs$460 = eval_mrs_regions();
-  bpf_ctx = get_mem_region(0U, mrs$460);
+  int f$462;
+  mrs$458 = eval_mrs_regions();
+  bpf_ctx = get_mem_region(0U, mrs$458);
   upd_reg(1U, (*bpf_ctx).start_addr);
-  bpf_interpreter_aux(fuel$458);
-  f$464 = eval_flag();
-  if (f$464 == 1) {
+  bpf_interpreter_aux(fuel$456);
+  f$462 = eval_flag();
+  if (f$462 == 1) {
     return eval_reg(0U);
   } else {
     return 0LLU;
