simulation/correct_eval_mrs_num.v
@@ -8,36 +8,36 @@ From bpf.proof Require Import Clightlogic MatchState CorrectRel CommonLemma.
 
 From bpf.clight Require Import interpreter.
 
+
 (**
-static struct memory_region *eval_mrs_regions(struct bpf_state* st){
-  return ( *st).mrs;
+static __attribute__((always_inline)) inline unsigned int eval_mrs_num(struct bpf_state* st){
+  return ( *st).mrs_num;
 }
 
-Print eval_mrs_regions.
-eval_mrs_regions = 
-fun st : stateM => Some (DxState.eval_mem_regions st, st)
-     : M MyMemRegionsType
+Print eval_mrs_num.
+eval_mrs_num = fun st : State.state => Some (eval_mem_num st, st)
+     : M nat
 
 *)
 
-Section Eval_mrs_regions.
+Section Eval_mrs_num.
 
   (** The program contains our function of interest [fn] *)
   Definition p : Clight.program := prog.
 
   (* [Args,Res] provides the mapping between the Coq and the C types *)
   Definition args : list Type := [].
-  Definition res : Type := (MyMemRegionsType:Type).
+  Definition res : Type := (nat:Type).
 
   (* [f] is a Coq Monadic function with the right type *)
-  Definition f : arrow_type args (M res) := eval_mrs_regions.
+  Definition f : arrow_type args (M res) := eval_mrs_num.
 
   Variable state_block: block. (**r a block storing all rbpf state information? *)
   Variable mrs_block: block.
   Variable ins_block: block.
 
   (* [fn] is the Cligth function which has the same behaviour as [f] *)
-  Definition fn: Clight.function := f_eval_mrs_regions.
+  Definition fn: Clight.function := f_eval_mrs_num.
 
   Definition stateM_correct (st:unit) (v: val) (stm:State.state) (m: Memory.Mem.mem) :=
     v = Vptr state_block Ptrofs.zero /\ match_state state_block mrs_block ins_block stm m.
@@ -48,9 +48,9 @@ Section Eval_mrs_regions.
                 (DList.DNil _)).
 
   (* [match_res] relates the Coq result and the C result *)
-  Definition match_res : res -> val -> State.state -> Memory.Mem.mem -> Prop := fun re v st m => re = (bpf_mrs st) /\ match_region_list mrs_block re v st m /\ match_state state_block mrs_block ins_block st m.
+  Definition match_res : res -> val -> State.state -> Memory.Mem.mem -> Prop := fun re v st m => mrs_correct re v st m /\ re = (mrs_num st) /\ match_state state_block mrs_block ins_block st m.
 
-  Instance correct_function3_eval_mrs_regions : forall a, correct_function3 p args res f fn (nil) false match_arg_list match_res a.
+  Instance correct_function3_eval_mrs_num : forall a, correct_function3 p args res f fn (nil) false match_arg_list match_res a.
   Proof.
     correct_function_from_body args.
     correct_body.
@@ -65,21 +65,19 @@ Section Eval_mrs_regions.
     subst v.
 
     assert (Hst' := Hst).
-    destruct Hst'. clear - Hst p0 mem_regs.
+    destruct Hst'. clear - Hst p0 mmrs_num.
 
     eexists. exists m, Events.E0.
 
     split.
     {
       repeat forward_star.
-
       rewrite Ptrofs.add_zero_l.
-      unfold Coqlib.align, AST.Mptr; simpl.
+      unfold Coqlib.align; simpl.
 
-      destruct mem_regs as (mem_regs & _).
-      rewrite <- mem_regs.
-      unfold AST.Mptr.
-      simpl.
+      destruct mmrs_num as (mmrs_num & _).
+      unfold Mem.loadv in mmrs_num.
+      rewrite mmrs_num.
       reflexivity.
       reflexivity.
     }
@@ -87,25 +85,18 @@ Section Eval_mrs_regions.
     {
       unfold match_res.
       split.
-      unfold State.eval_mem_regions.
-      reflexivity.
-      split;[ | assumption].
-      unfold match_region_list, Ptrofs.zero, State.eval_mem_regions.
-      split; [reflexivity |].
-      split; [reflexivity |].
-      destruct mem_regs as ( _ & Hmrs).
-      unfold match_regions in Hmrs.
-      destruct Hmrs as (Hlen & _ & Hmrs).
-      split; assumption.
+      - unfold mrs_correct, eval_mem_num.
+        split; [reflexivity | ].
+        lia.
+      - split.
+        unfold eval_mem_num.
+        reflexivity.
+        assumption.
     }
 
-    split.
-    simpl.
-    constructor.
-    simpl.
-    split; reflexivity.
+    split; [simpl; constructor; reflexivity | split; reflexivity].
   Qed.
 
-End Eval_mrs_regions.
+End Eval_mrs_num.
 
-Existing Instance correct_function3_eval_mrs_regions.
+Existing Instance correct_function3_eval_mrs_num.
