simulation/correct_is_well_chunk_bool.v
@@ -13,66 +13,66 @@ From bpf.clight Require Import interpreter.
 
 Section Is_well_chunk_bool.
 
-Variable st_block : block.
-Variable mrs_block: block.
-Variable ins_block: block.
+  Variable st_block : block.
+  Variable mrs_block: block.
+  Variable ins_block: block.
 
-(** The program contains our function of interest [fn] *)
-Definition p : Clight.program := prog.
+  (** The program contains our function of interest [fn] *)
+  Definition p : Clight.program := prog.
 
-(* [Args,Res] provides the mapping between the Coq and the C types *)
-Definition args : list Type := [memory_chunk:Type].
-Definition res : Type := bool.
+  (* [Args,Res] provides the mapping between the Coq and the C types *)
+  Definition args : list Type := [memory_chunk:Type].
+  Definition res : Type := bool.
 
-(* [f] is a Coq Monadic function with the right type *)
-Definition f := is_well_chunk_bool.
+  (* [f] is a Coq Monadic function with the right type *)
+  Definition f := is_well_chunk_bool.
 
-(* [fn] is the Cligth function which has the same behaviour as [f] *)
-Definition fn: Clight.function := f_is_well_chunk_bool.
+  (* [fn] is the Cligth function which has the same behaviour as [f] *)
+  Definition fn: Clight.function := f_is_well_chunk_bool.
 
-Definition match_state (st_block : block) (_ : unit) (v : val) (st: State.state) (m : Memory.Mem.mem) : Prop :=
-  v = Vptr st_block Ptrofs.zero /\ match_state st_block mrs_block ins_block st m.
+  Definition stateM_correct (st_block : block) (_ : unit) (v : val) (st: State.state) (m : Memory.Mem.mem) : Prop :=
+    v = Vptr st_block Ptrofs.zero /\ match_state st_block mrs_block ins_block st m.
 
-Ltac exec_seq_of_labeled_statement :=
-  match goal with
-  | |- context[seq_of_labeled_statement ?X] =>
-      let x := (eval simpl in (seq_of_labeled_statement X)) in
-      change (seq_of_labeled_statement X) with x
-  end.
+  Ltac exec_seq_of_labeled_statement :=
+    match goal with
+    | |- context[seq_of_labeled_statement ?X] =>
+        let x := (eval simpl in (seq_of_labeled_statement X)) in
+        change (seq_of_labeled_statement X) with x
+    end.
 
-Instance correct_function_is_well_chunk_bool2 : forall a, correct_function3
-    p args res f fn nil true (DList.DCons  (stateless match_chunk) (DList.DNil _)) (stateless match_bool) a.
-Proof.
-  correct_function_from_body args.
-  correct_body.
-  unfold INV, f.
-  repeat intro.
-  simpl in *.
-  destruct (is_well_chunk_bool c st) eqn: Heq; [idtac | constructor].
-  destruct p0 as (v',st'); intros.
+  Instance correct_function_is_well_chunk_bool2 : forall a, correct_function3
+      p args res f fn nil true (DList.DCons  (stateless match_chunk) (DList.DNil _)) (stateless match_bool) a.
+  Proof.
+    correct_function_from_body args.
+    correct_body.
+    unfold INV, f.
+    repeat intro.
+    simpl in *.
+    destruct (is_well_chunk_bool c st) eqn: Heq; [idtac | constructor].
+    destruct p0 as (v',st'); intros.
 
-  get_invariant _chunk.
-  unfold stateless, match_chunk in c0.
-  subst.
+    get_invariant _chunk.
+    unfold stateless, match_chunk in c0.
+    subst.
 
-  exists (Vint (if v' then Integers.Int.one else Integers.Int.zero)).
-  exists m, Events.E0.
-  
-  repeat split; unfold step2.
-  -
-    unfold memory_chunk_to_valu32, well_chunk_Z in p0.
-    unfold align_chunk in p0.
-    destruct c; inv Heq; simpl.
-    all: try
-    forward_star; forward_star;
-    [ rewrite Int.unsigned_repr; [idtac | rewrite Int_max_unsigned_eq64; lia]; simpl; forward_star |
-    repeat forward_star | reflexivity].
-  - simpl.
-    constructor.
-    destruct v' ; reflexivity.
-  - unfold is_well_chunk_bool, returnM in Heq.
-    destruct c; inversion Heq; reflexivity.
-Qed.
+    exists (Vint (if v' then Integers.Int.one else Integers.Int.zero)).
+    exists m, Events.E0.
+    
+    repeat split; unfold step2.
+    -
+      unfold memory_chunk_to_valu32, well_chunk_Z in p0.
+      unfold align_chunk in p0.
+      destruct c; inv Heq; simpl.
+      all: try
+      forward_star; forward_star;
+      [ rewrite Int.unsigned_repr; [idtac | rewrite Int_max_unsigned_eq64; lia]; simpl; forward_star |
+      repeat forward_star | reflexivity].
+    - simpl.
+      constructor.
+      destruct v' ; reflexivity.
+    - unfold is_well_chunk_bool, returnM in Heq.
+      destruct c; inversion Heq; reflexivity.
+  Qed.
 
 End Is_well_chunk_bool.
 
