simulation/correct_check_mem.v
@@ -1,0 +1,420 @@
+From bpf.comm Require Import MemRegion State Monad.
+From bpf.monadicmodel Require Import rBPFInterpreter.
+From dx.Type Require Import Bool.
+From dx Require Import IR.
+From Coq Require Import List ZArith.
+From compcert Require Import Integers Values Clight Memory AST.
+From compcert Require Import Coqlib.
+Import ListNotations.
+
+From bpf.proof Require Import clight_exec Clightlogic CorrectRel MatchState CommonLemma.
+
+From bpf.clight Require Import interpreter.
+
+From bpf.simulation Require Import correct_is_well_chunk_bool correct_eval_mrs_num correct_eval_mrs_regions correct_check_mem_aux correct_cmp_ptr32_nullM.
+
+(**
+Check check_mem.
+check_mem
+     : permission -> memory_chunk -> val -> M val
+*)
+
+Section Check_mem.
+
+  (** The program contains our function of interest [fn] *)
+  Definition p : Clight.program := prog.
+
+  (* [Args,Res] provides the mapping between the Coq and the C types *)
+  (* Definition Args : list CompilableType := [stateCompilableType].*)
+  Definition args : list Type := [(permission:Type); (memory_chunk:Type); (val:Type)].
+  Definition res : Type := (val:Type).
+
+  (* [f] is a Coq Monadic function with the right type *)
+  Definition f : arrow_type args (M res) := check_mem.
+
+  Variable state_block: block. (**r a block storing all rbpf state information? *)
+  Variable mrs_block: block.
+  Variable ins_block: block.
+
+  (* [fn] is the Cligth function which has the same behaviour as [f] *)
+  Definition fn: Clight.function := f_check_mem.
+
+  Definition stateM_correct (st:unit) (v: val) (stm:State.state) (m: Memory.Mem.mem) :=
+    v = Vptr state_block Ptrofs.zero /\ match_state state_block mrs_block ins_block stm m.
+
+  (* [match_arg] relates the Coq arguments and the C arguments *)
+  Definition match_arg_list : DList.t (fun x => x -> val -> State.state -> Memory.Mem.mem -> Prop) ((unit:Type) ::args) :=
+    DList.DCons stateM_correct
+      (DList.DCons (stateless perm_correct)
+        (DList.DCons (stateless match_chunk)
+          (DList.DCons (stateless valu32_correct)
+            (DList.DNil _)))).
+
+  (* [match_res] relates the Coq result and the C result *)
+  Definition match_res : res -> val -> State.state -> Memory.Mem.mem -> Prop := fun x v st m => x = v /\ ((exists b ofs, x = Vptr b ofs) \/ v = Vint (Int.zero)) /\ match_state state_block mrs_block ins_block st m.
+(*
+Ltac build_app_aux T :=
+  match T with
+  | ?F ?X => let ty := type of X in
+             let r := build_app_aux F in
+             constr:((mk ty X) :: r)
+  | ?X    => constr:(@nil dpair)
+  end.
+
+Ltac get_function T :=
+  match T with
+  | ?F ?X => get_function F
+  | ?X    => X
+  end.
+
+Ltac build_app T :=
+  let a := build_app_aux T in
+  let v := (eval simpl in (DList.of_list_dp (List.rev a))) in
+  let f := get_function T in
+  match type of v with
+  | DList.t _ ?L =>
+      change T with (app (f: arrow_type L _) v)
+  end.
+
+Ltac change_app_for_body :=
+  match goal with
+  | |- @correct_body _ _ ?F _ _ _ _ _ _ _ _
+    => build_app F
+  end.
+
+Ltac change_app_for_statement :=
+  match goal with
+  | |- @correct_statement _ _ ?F _ _ _ _ _ _ _ _
+    => build_app F
+  end.
+*)
+  Instance correct_function3_check_mem : forall a, correct_function3 p args res f fn (nil) false match_arg_list match_res a.
+  Proof.
+    correct_function_from_body args.
+    correct_body.
+    (** how to use correct_* *)
+    unfold INV.
+    unfold f, app.
+    unfold check_mem.
+    eapply correct_statement_seq_body with (modifies1:=nil).
+    change_app_for_statement.
+    eapply correct_statement_call with (has_cast := true).
+
+    my_reflex.
+    reflexivity.
+    reflexivity.
+    typeclasses eauto.
+    { unfold INV.
+      unfold var_inv_preserve.
+      intros.
+      unfold match_temp_env in *.
+      rewrite Forall_fold_right in *.
+      simpl in *.
+      intuition. subst m' st'. assumption.
+    }
+
+    reflexivity.
+    reflexivity.
+    reflexivity.
+    prove_in_inv.
+    prove_in_inv.
+    reflexivity.
+    reflexivity.
+
+    intros.
+    change (match_temp_env INV le st m) in H.
+    unfold INV in H.
+    get_invariant _chunk.
+    unfold stateless, match_chunk in c2.
+    subst v.
+    exists (rBPFAST.memory_chunk_to_valu32 c0::nil).
+    split.
+    unfold map_opt, exec_expr. rewrite p0.
+    reflexivity.
+    intros. simpl.
+    unfold stateless, match_chunk.
+    tauto.
+
+    intros.
+    eapply correct_statement_if_body; [prove_in_inv | destruct x ]. 2:{ (**r if-else branch *)
+    unfold correct_body.
+    intros.
+    unfold returnM.
+    intros.
+    exists (Vint (Int.repr 0)), m0, Events.E0.
+    split.
+    {
+      forward_star.
+      forward_star.
+    }
+    split.
+    {
+      unfold match_res, Vnullptr, Int.zero; simpl.
+      split; [reflexivity | ].
+      split.
+      right.
+      reflexivity.
+      get_invariant _st.
+      unfold stateM_correct in c2.
+      destruct c2 as (_ & c2); assumption.
+    }
+    split;[ constructor; reflexivity | ].
+    instantiate (1 := nil).
+    split; reflexivity.
+    }
+    (**r if-then branch *)
+
+    eapply correct_statement_seq_body with (modifies1:=nil).
+    change_app_for_statement.
+    eapply correct_statement_call with (has_cast := false).
+    my_reflex.
+    reflexivity.
+    reflexivity.
+    typeclasses eauto.
+    { unfold INV.
+      unfold var_inv_preserve.
+      intros.
+      unfold match_temp_env in *.
+      rewrite Forall_fold_right in *.
+      simpl in *.
+      destruct H; subst.
+      intuition.
+    }
+    reflexivity.
+    reflexivity.
+    reflexivity.
+    prove_in_inv.
+    prove_in_inv.
+    reflexivity.
+    reflexivity.
+
+    unfold INV; intro H.
+    correct_Forall.
+    get_invariant _st.
+    unfold stateM_correct in c2.
+    destruct c2 as (Hc2_eq & Hst); subst.
+    exists (Vptr state_block Ptrofs.zero::nil).
+    split.
+    unfold map_opt,exec_expr.
+    rewrite p0.
+    reflexivity.
+    simpl. intros.
+    instantiate (1 := ins_block).
+    instantiate (1 := mrs_block).
+    instantiate (1 := state_block).
+    unfold correct_eval_mrs_num.stateM_correct.
+    split; [| constructor].
+    split; [ reflexivity | assumption ].
+
+    intros.
+    eapply correct_statement_seq_body with (modifies1:=nil).
+    change_app_for_statement.
+    eapply correct_statement_call with (has_cast := false).
+    my_reflex.
+    reflexivity.
+    reflexivity.
+    typeclasses eauto.
+    { unfold INV.
+      unfold var_inv_preserve.
+      intros.
+      unfold match_temp_env in *.
+      rewrite Forall_fold_right in *.
+      simpl in *.
+      destruct H; subst.
+      intuition.
+    }
+    reflexivity.
+    reflexivity.
+    reflexivity.
+    prove_in_inv.
+    prove_in_inv.
+    reflexivity.
+    reflexivity.
+
+    unfold INV; intro H.
+    correct_Forall.
+    get_invariant _st.
+    unfold stateM_correct in c2.
+    destruct c2 as (Hc2_eq & Hst); subst.
+    exists (Vptr state_block Ptrofs.zero::nil).
+    split.
+    unfold map_opt, exec_expr.
+    rewrite p0; reflexivity.
+    simpl;intros.
+    instantiate (1 := ins_block).
+    instantiate (1 := mrs_block).
+    instantiate (1 := state_block).
+    unfold correct_eval_mrs_num.stateM_correct.
+    split; [| constructor].
+    split; [ reflexivity | assumption ].
+
+    intros.
+    eapply correct_statement_seq_body with (modifies1:=nil).
+    change_app_for_statement.
+    eapply correct_statement_call with (has_cast := false).
+    my_reflex.
+    reflexivity.
+    reflexivity.
+    typeclasses eauto.
+    { unfold INV.
+      unfold var_inv_preserve.
+      intros.
+      unfold match_temp_env in *.
+      rewrite Forall_fold_right in *.
+      simpl in *.
+      destruct H; subst.
+      intuition.
+    }
+    reflexivity.
+    reflexivity.
+    reflexivity.
+    prove_in_inv.
+    prove_in_inv.
+    reflexivity.
+    reflexivity.
+
+    unfold INV; intro H.
+    correct_Forall.
+    get_invariant _st.
+    get_invariant _mem_reg_num.
+    get_invariant _perm.
+    get_invariant _chunk.
+    get_invariant _addr.
+    get_invariant _mrs.
+    unfold stateM_correct in c2.
+    destruct c2 as (Hv_eq & Hst).
+    unfold correct_eval_mrs_num.match_res in c3.
+    destruct c3 as (Hc_eq & _).
+    unfold stateless, perm_correct in c4.
+    unfold stateless, match_chunk in c5.
+    unfold stateless, valu32_correct in c6.
+    destruct c6 as (Hc1_eq & vi & Hvi_eq).
+    unfold correct_eval_mrs_regions.match_res in c7.
+    destruct c7 as (Hx0_eq & Hmrs & _).
+    subst.
+    exists ((Vptr state_block Ptrofs.zero) ::
+            v0 :: v1 :: 
+            (rBPFAST.memory_chunk_to_valu32 c0) ::
+            (Vint vi) :: v4 ::
+            nil).
+    split.
+    unfold map_opt, exec_expr.
+    rewrite p0, p1, p2, p3, p4, p5; reflexivity.
+    simpl;intros.
+    instantiate (1 := mrs_block).
+    instantiate (1 := ins_block).
+    instantiate (1 := state_block).
+    unfold correct_check_mem_aux.stateM_correct.
+    split; [| constructor].
+    split; [ reflexivity | assumption ].
+    assumption.
+    unfold stateless, perm_correct, match_chunk, valu32_correct.
+    split; [assumption |].
+    split; [reflexivity |].
+    split; [split; [reflexivity | eexists; reflexivity] |].
+    split; [ assumption |constructor].
+
+    intros.
+    eapply correct_statement_seq_body with (modifies1:=nil);eauto.
+    unfold typeof.
+    change_app_for_statement.
+    eapply correct_statement_call with (has_cast:=true).
+    my_reflex.
+    reflexivity.
+    reflexivity.
+    intros.
+    typeclasses eauto.
+    { unfold INV.
+      unfold var_inv_preserve.
+      intros.
+      unfold match_temp_env in *.
+      rewrite Forall_fold_right in *.
+      simpl in *.
+      destruct H; subst.
+      intuition.
+    }
+    reflexivity.
+    reflexivity.
+    reflexivity.
+    prove_in_inv.
+    prove_in_inv.
+    reflexivity.
+    reflexivity.
+
+    unfold INV; intro H.
+    correct_Forall.
+    get_invariant _st.
+    get_invariant _check_mem__1.
+    exists (v::v0::nil).
+    split.
+    unfold map_opt, exec_expr.
+    rewrite p0, p1; reflexivity.
+    simpl;intros.
+    intuition eauto.
+    unfold val_ptr_null_correct.
+    unfold correct_check_mem_aux.match_res in c3.
+    change Vnullptr with (Vint Int.zero).
+    destruct c3 as (Hv0_eq & Hptr & Hst).
+    subst.
+    split; [reflexivity | ].
+    intuition eauto.
+
+    intros.
+    eapply correct_statement_if_body; [prove_in_inv | destruct x2 ]. 2:{
+      unfold correct_body, returnM.
+      intros.
+      unfold INV in H.
+      get_invariant _check_mem__1.
+      unfold correct_check_mem_aux.match_res in c2.
+      destruct c2 as (Hv_eq & Hptr & Hst).
+      subst.
+      exists v, m4, Events.E0.
+      instantiate (1 := nil).
+      destruct Hptr as [ (b & ofs & Hptr) | Hnull].
+      - rewrite Hptr.
+        split.
+        forward_star.
+        unfold Cop.sem_cast; simpl.
+        rewrite Hptr.
+        reflexivity.
+        rewrite Hptr.
+        forward_star.
+        split.
+        unfold match_res.
+        split; [reflexivity | ].
+        split; [left; eexists; eexists; reflexivity | assumption].
+        split; [constructor; reflexivity | split; reflexivity].
+      - rewrite Hnull.
+        split.
+        forward_star.
+        rewrite Hnull.
+        reflexivity.
+        rewrite Hnull.
+        forward_star.
+        split.
+        unfold match_res.
+        split; [reflexivity | ].
+        split; [right; reflexivity | assumption].
+        split; [constructor; reflexivity | split; reflexivity].
+    }
+    eapply correct_body_Sreturn_Some; eauto.
+    intros.
+    split.
+    unfold exec_expr; simpl.
+    reflexivity.
+    split.
+    unfold match_res, Vnullptr, Int.zero; simpl.
+    split; [reflexivity |].
+    get_invariant _st.
+    unfold stateM_correct in c2.
+    destruct c2 as (_ & Hst).
+    split; [right; reflexivity | assumption].
+    reflexivity.
+
+    intuition.
+    all: reflexivity.
+  Qed.
+
+End Check_mem.
+
+Existing Instance correct_function3_check_mem.
